theories/ordinals/Ackermann/wConsistent.v
@@ -14,14 +14,14 @@ Lemma wCon2Con : forall T : System, wConsistent T -> Consistent LNN T.
 Proof.
   intros T H; unfold wConsistent in H.
   unfold Consistent, Inconsistent; 
-    assert (H0: SysPrf T (exH 0, ~ ~ v_ 0 = v_ 0)%nn) 
+    assert (H0: SysPrf T (exH 0, ~ ~ v#0 = v#0)%nn) 
     by apply existSimp, nnI, eqRefl.
   assert
     (H1 : forall x : nat,
-        In x (freeVarFormula LNN (v_ 0 <> v_ 0)%nn) -> 0 = x)
+        In x (freeVarFormula LNN (v#0 <> v#0)%nn) -> 0 = x)
     by (intros x H1; simpl in H1; repeat induction H1; auto).
   destruct  (H _ _ H1 H0) as [x H2]; 
-    now exists (substituteFormula LNN (v_ 0 <> v_ 0)%nn 0
+    now exists (substituteFormula LNN (v#0 <> v#0)%nn 0
                   (natToTerm x)).
 Qed.
 
