theories/ordinals/MoreAck/FolExamples.v
@@ -38,7 +38,7 @@ Lemma eq_refl : forall L (t:Term L), Prf L nil (t = t)%fol.
 (* end snippet eqRefl *)
 Proof. 
   intros L t.
-  assert (H: Prf L nil (forallH 0 (v_ 0 = v_ 0))%fol). 
+  assert (H: Prf L nil (forallH 0 (v#0 = v#0))%fol). 
   {
     apply GEN.
     - cbn; auto. 
@@ -47,7 +47,7 @@ Proof.
   change (nil:(list (Formula L))) with (nil++nil: list(Formula L)).
   eapply MP.
   2: apply H.
-  generalize (FA1 _ (v_ 0 = v_ 0)%fol 0 t).
+  generalize (FA1 _ (v#0 = v#0)%fol 0 t).
   intro; assumption.   
 Qed. 
 
@@ -148,18 +148,19 @@ Example F3 : Formula L :=
   Notation P t := (atomic L P_ (Tcons t Tnil)).
   Notation R t1 t2 :=
     (@atomic L R_ (Tcons t1 (Tcons t2 Tnil))).
+
+Example F4: Formula L := (v#0 = a \/ exH 1, v#0 = f v#1)%fol. 
+Example F5: Formula L := (v#0 = a \/ v#0 = f v#1)%fol. 
 (* end snippet toyNotationForm *)
 
 
 (* begin snippet toyNotationForm2 *)
-Print F2.
-
 Goal F1 = (R a b)%fol. Proof refl_equal. 
 
-Goal F2 = (allH 0 1, R v_ 0 v_ 1 -> R v_ 1 v_ 0)%fol. 
+Goal F2 = (allH 0 1, R v#0 v#1 -> R v#1 v#0)%fol. 
 Proof refl_equal.
 
-Goal F3 = (allH 0, v_ 0 = a \/ exH 1, v_ 0 = f v_ 1)%fol.  
+Goal F3 = (allH 0, v#0 = a \/ exH 1, v#0 = f v#1)%fol.  
 Proof refl_equal.
 
 (** The following computation expands some derived connectives and 
@@ -174,7 +175,7 @@ Proof.  reflexivity. Qed.
 (* end snippet toyNotationForm2 *)
 
 (* begin snippet boundVars *)
-Goal (allH 1, v_ 1 = a)%fol <> (allH 0, v_ 0 = a)%fol.
+Goal (allH 1, v#1 = a)%fol <> (allH 0, v#0 = a)%fol.
   discriminate. 
 Qed. 
 (* end snippet boundVars *)
@@ -186,7 +187,7 @@ Goal apply L a_ Tnil = a.
 Proof. reflexivity. Qed. 
 
 (** f a **)
-Goal apply L f_  (Tcons  (apply L a_ Tnil) Tnil) = (f a). 
+Goal apply L f_  (Tcons  (apply L a_ Tnil) Tnil) = f a. 
 Proof. reflexivity. Qed. 
 
 (** f (f v1) **)
@@ -202,16 +203,38 @@ Proof. reflexivity. Qed.
 
 Check (f a)%fol. 
 
+(* begin snippet DepthCompute *)
+
+(* end snippet DepthCompute *)
+
+(* begin snippet ltDepth1:: no-out *)
+Goal lt_depth _ F1 F2. 
+cbn. red.  compute; auto with arith. 
+Qed.
+(* end snippet ltDepth1 *)
+
+(* begin snippet freeVarExamples *)
+Compute  freeVarFormula _ F5.
+
+Compute List.nodup Nat.eq_dec (freeVarFormula _ F5).
+
+Compute freeVarFormula _ (close _ F5).
+
+Compute substituteFormula L F5 0 (f a).
+(* end snippet freeVarExamples *)
 
 
-Example f3 := (v_ 0 = a \/ exH 1, (v_ 0 = f (v_ 1)))%fol.
+Locate f. 
 
-Compute substituteFormula L f3 0 (g (v_ 1))%fol. 
 
-Goal substituteFormula L f3 0 (g (v_ 1))%fol =
-       (g (v_ 1) = a \/ exH 2, (g (v_ 1) = f (v_ 2)))%fol.
-reflexivity. 
-Qed. 
+(* begin snippet substNotStructural *)
+Section OnSubstF.
+  Let G : Formula L := (v#1 <> f v#2)%fol.
+ Let F : Formula L := (exH 2, G)%fol.
+ Compute substF L  F 1 (f v#2)%fol. 
+ Compute (exH 2, substF L G 1 (f v#2))%fol.
+End OnSubstF.  
+(* end snippet substNotStructural *)
 
 Lemma MP' f g H1 H2 H: H = H1 ++ H2 -> Prf L H1 (f -> g)%fol ->
                         Prf L H2 f ->  Prf L H g.
@@ -283,7 +306,7 @@ Section Drinkers_theorem.
 
  Lemma D0 : forall i, 
       SysPrf _ (Empty_set _)
-        ( ~ forallH i (P (v_ i)) -> exH i, (~ (P (v_ i))))%fol. 
+        ( ~ forallH i (P (v#i)) -> exH i, (~ (P (v#i))))%fol. 
 Proof.
     intro i; apply cp2, impI, forallI. 
     - intros [f [H H0]]; inversion H0. 
@@ -293,8 +316,8 @@ Proof.
       + inversion H. 
       + now destruct n. 
     - apply nnE; 
-        assert (H:(~ ~ (P (v_ i)))%fol = (* clumsy *)
-                  (substituteFormula _ (~ ~ (P (v_ i))) i (v_ i))%fol). 
+        assert (H:(~ ~ (P (v#i)))%fol = (* clumsy *)
+                  (substituteFormula _ (~ ~ (P (v#i))) i (v#i))%fol). 
       { cbn; destruct (Nat.eq_dec i) as [_ | n].
         auto. 
         now destruct n. 
@@ -304,8 +327,8 @@ Proof.
   Qed. 
   
   Lemma D01 T i : SysPrf _ T
-                    (~ forallH i (P (v_ i)) -> 
-                      exH i, (~ (P (v_ i))))%fol. 
+                    (~ forallH i (P (v#i)) -> 
+                      exH i, (~ (P (v#i))))%fol. 
   Proof. 
     apply sysExtend with (Empty_set _).
     - red; destruct 1.   
@@ -313,17 +336,17 @@ Proof.
   Qed. 
 
   Let f : Formula L :=
-        (exH 0, (P (v_ 0) -> forallH 1 (P (v_ 1))))%fol. 
+        (exH 0, (P (v#0) -> forallH 1 (P (v#1))))%fol. 
 
   Theorem drinkers_thm : SysPrf L (Empty_set _) f. 
   Proof with auto with sets.  
-    pose (F := forallH 1 (P (v_ 1))%fol).
+    pose (F := forallH 1 (P (v#1))%fol).
     unfold f; eapply orE with (notH F) F; [apply noMiddle | | ].
     - apply impI;
       assert (SysPrf L (Add (Empty_set _) (~ F)%fol) 
-                (exH 1, (~ (P (v_ 1))))%fol).  
-      { replace (exH 1, (~ (P (v_ 1))))%fol  
-          with (~ (forallH 1 (~ (~  (P (v_ 1))))))%fol. 
+                (exH 1, (~ (P (v#1))))%fol).  
+      { replace (exH 1, (~ (P (v#1))))%fol  
+          with (~ (forallH 1 (~ (~  (P (v#1))))))%fol. 
         - unfold F; eapply impE. 
           + eapply D01. 
           + apply Axm; right; split. 
@@ -338,18 +361,20 @@ Proof.
              subst; now simpl in H0. 
         * cbn; auto. 
         * eapply H. 
-        * apply impI; eapply existI with (v_ 1)%fol.
+        * apply impI; eapply existI with (v#1)%fol.
           cbn; apply impI. 
-          eapply contradiction with (P (v_ 1))%fol.  
+          eapply contradiction with (P (v#1))%fol.  
           -- apply Axm; red ...
           -- apply Axm; red ...   
-    - apply impI; apply existI with (v_ 0)%fol. 
+    - apply impI; apply existI with (v#0)%fol. 
       cbn;  apply impI. 
       apply Axm; red; auto with sets. 
   Qed. 
 
 
 End Drinkers_theorem. 
+
+
 
 End Toy.
 
@@ -396,29 +421,6 @@ About Formula_rect.
 (* end snippet FormulaRect *)
 
 (** depth-order vs structural order *)
-(* begin snippet DepthCompute *)
-Compute depth _ f1.
-(* end snippet DepthCompute *)
-
-(* begin snippet ltDepth1:: no-out *)
-Goal lt_depth _ f2 f1. 
-cbn. red; auto with arith. 
-Qed.
-(* end snippet ltDepth1 *)
-
-(* begin snippet freeVarExamples *)
-Compute  freeVarFormula _ f2.
-
-Compute List.nodup Nat.eq_dec (freeVarFormula _ f3).
-
-Compute close _ f3.
-
-Compute freeVarFormula _ f3.
-
-Compute freeVarFormula _ (close _ f3).
-
-Compute substituteFormula LNN f3 0 (apply LNN Zero_ (Tnil)) . 
-(* end snippet freeVarExamples *)
 
 Section depth_rec_demo. 
 Variable L: Language.
